mrdt.fst
@@ -1,7 +1,0 @@
-module Mrdt
-
-open FStar.List.Tot
-
-class mrdt (state:eqtype) (operation:eqtype) = {
-  apply_op : state -> operation -> state;
-}
